\documentclass[10pt]{article}
\usepackage[margin = 0.5 in]{geometry}
\usepackage{amsmath}
\usepackage{amssymb}
\usepackage{multicol}

\AtBeginEnvironment{align}{\setcounter{equation}{0}}
\setlength{\columnsep}{0.5in}
\setlength{\parindent}{0in}

\title{Table of Laplace Transforms}
\begin{document}

% \begin{multicols*}{2}
\textbf{Table of Laplace Transforms}

\begin{align}
    L[k] &= \frac{k}{s} \\
    L[t^n] &= \frac{n!}{s^{n+1}} \\
    L[e^{at}] &= \frac{1}{s - a}\\
    L[t^n e^{at}] &= \frac{n!}{(s-a)^{n+1}} \\
    L[\cos(kt)] &= \frac{s}{s^2 + k^2} \\
    L[\sin(kt)] &= \frac{k}{s^2 + k^2} \\
    L[e^{at} \cos(kt)] &= \frac{s - a}{(s - a)^2 + k^2} \\
    L[e^{at} \sin(kt)] &= \frac{k}{(s - a)^2 + k^2} \\
    L[t \sin(kt)] &= \frac{2ks}{(s^2 + k^2)^2} \\
    L[t \cos(kt)] &= \frac{s^2 - k^2}{(s^2 + k^2)^2}\\
    L[t \sin(kt+a)] &= \frac{s\sin(a) + k \cos(a)}{s^2 + k^2} \\
    L[t \cos(kt + a)] &= \frac{s \cos(a) - k \sin(a)}{s^2 + k^2} \\
    L[u(t-a)] &= \frac{e^{-as}}{s}, a \geq 0
\end{align}

\textbf{Differentiation Properties}

If \( L[y(t)] = Y(s) \), then:

\begin{align}
    L[y'(t)] &= sY(s) - y(0) \\
    L[y''(t)] &= s^2 Y(s) - sy(0) - y'(0)
\end{align}

\textbf{Shifting Theorems}

\textbf{First Shifting Theorem}
If \( L[f(t)] = F(s) \), then:
\begin{align}
    L[e^{at} f(t)] &= F(s - a)
\end{align}


\textbf{Second Shifting Theorem}
If \( L[f(t)] = F(s) \), then:
\begin{align}
    L[u(t - a) \cdot f(t - a)] &= e^{-as} \cdot L[f(t)] \\ 
                                &= e^{-as} F(s) \\
    L^{-1}[e^{-as} F(s)] &= u(t - a) \cdot f(t - a)
\end{align}

\textbf{Laplace Transforms of Piecewise Functions}

Suppose \( f(t) \) is a piecewise-defined function:
\[
f(t) = \begin{cases} 
      f_1(t) & 0 \leq t < a_1 \\
      f_2(t) & a_1 \leq t < a_2 \\
      f_2(t) & a_2 \leq t < a_3 \\
        ... & ... \\ 
      f_n(t) & a_{n-1} \leq t < a_n \\
   \end{cases}
\]

f(t) can be wrtten in termss of step functions as:
\[
f(t) = f_1(t) + (f_2(t) - f_1(t)) u(t - a) + (f_3(t) - f_2(t)) u(t - a_2) + ... + (f_n(t) - f_{n-1}(t)) u(t - a_{n-1})
\]


% \end{multicols*}

\end{document}
